Jessie: valid_inv axiom now contains the invariant
git-svn-id: https://www.lri.fr/svn/demons/why2/trunk@2171 ecafba89-7d34-45a1-8a0b-92829e960b72

jc/jc_interp.ml
@@ -522,17 +522,21 @@ let tr_valid_inv st acc =
     List.fold_left (fun acc (name, fi) ->
       (name, memory_field fi)::acc) acc st.jc_struct_info_fields)
     Jc_norm.structs_table [] in
-  let memories = List.sort (fun (name1, _) (name2, _) -> compare name2 name1) memories in
+  let memories = List.sort (fun (name1, _) (name2, _) ->
+    compare name2 name1) memories in
   let rec only_one prev acc = function
     [] -> acc
   | ((name, _) as x)::tl ->
       if name = prev then only_one prev acc tl
       else only_one name (x::acc) tl in
   let memories = only_one "" [] memories in
-  (**** valid_inv predicate ****)
+  (**** valid_inv predicate declaration ****)
   let valid_inv_type = simple_logic_type "prop" in
-  let vi_this = "???", { logic_type_name = "pointer" ; logic_type_args = [simple_logic_type st.jc_struct_info_name] } in
-  let logic = Logic(false, valid_inv_name st, vi_this::memories, valid_inv_type) in
+  let vi_this = "???",
+    { logic_type_name = "pointer" ;
+      logic_type_args = [simple_logic_type st.jc_struct_info_name] } in
+  let logic = Logic(false, valid_inv_name st, vi_this::memories,
+    valid_inv_type) in
   let acc = logic::acc
   in
   (**** valid_inv_sem axiom ****)
@@ -547,11 +551,14 @@ let tr_valid_inv st acc =
   let fields_valid_inv = List.map (fun (name, fi) ->
     match fi.jc_field_info_type with
     | JCTpointer(st, _, _) ->
-        LPred(valid_inv_name st, LApp("select", [LVar name; this_var])::memories_params)
+        LPred(valid_inv_name st,
+          LApp("select", [LVar name; this_var])::memories_params)
     | JCTnative _
     | JCTlogic _
     | JCTrange _ -> LTrue) st.jc_struct_info_fields in
-  let sem = LIff(LPred(valid_inv_name st, this_var::memories_params), make_and_list fields_valid_inv) in
+  let sem = LIff(LPred(valid_inv_name st, this_var::memories_params),
+    make_and (make_and_list fields_valid_inv)
+      (invariant_for_struct this_var st)) in
   (* quantifiers *)
   let sem = List.fold_left (fun acc (id, ty) ->
     LForall(id, ty, acc)) sem ((this, this_ty)::memories) in
